Better mutual wf rec doc

examples/mutualwfrec.v
@@ -1,54 +1,68 @@
+(* begin hide *)
+(**********************************************************************)
+(* Equations                                                          *)
+(* Copyright (c) 2009-2019 Matthieu Sozeau <matthieu.sozeau@inria.fr> *)
+(**********************************************************************)
+(* This file is distributed under the terms of the                    *)
+(* GNU Lesser General Public License Version 2.1                      *)
+(**********************************************************************)
+
 From Equations Require Import Equations.
-Require Import Lia.
-Set Equations Transparent.
-Equations evenodd (b : bool) (n : nat) : Prop by rec n lt :=
-  evenodd true 0 := True;
-  evenodd true (S n) := evenodd false n;
-  evenodd false 0 := False;
-  evenodd false (S n) := evenodd true n.
-
-Eval vm_compute in evenodd true 4.
-
+From Coq Require Import List Program.Syntax Arith Lia.
 Require Import List Wellfounded.
-Set Asymmetric Patterns.
+(* end hide *)
+(** * Mutual well-founded recursion using dependent pattern-matching
 
-Polymorphic Inductive ty : forall (A : Type) (P : A -> Type), Type :=
-| ty0 : ty nat (fun _ => nat)
-| ty1 : ty (list nat) (fun _ => bool).
+  We present a simple encoding of mutual recursion through the use of
+  dependent pattern-matching on a GADT-like representation of the functions
+  prototypes. We use a simple toy measure here to justify termination,
+  but more elaborate well-founded relations can be used as well.
+ *)
 
-Polymorphic Derive Signature NoConfusion for ty.
+Set Equations Transparent.
 
-
+(** Use nice notations for sigma types *)
 Notation "{ x : A & y }" := (@sigma A (fun x : A => y)%type) (x at level 99) : type_scope.
 Notation "{ x & y }" := (@sigma _ (fun x : _ => y)%type) (x at level 99) : type_scope.
-
 Notation "&( x , .. , y , z )" :=
   (@sigmaI _ _ x .. (@sigmaI _ _ y z) ..)
     (right associativity, at level 4,
      format "&( x ,  .. ,  y  ,  z )").
 
-Polymorphic Equations rel : {A &{ P &{ _ : A & ty A P }}} -> {A & { P & {_ : A & ty A P}}} -> Prop :=
-  rel &(A, P, a, ta) &(B, Q, b, tb) =>
-  match ta in ty A P, tb in ty B Q return A -> B -> Prop with
-  | ty0, ty0 => lt
-  | ty1, ty1 => fun l l' => length l < length l'
-  | ty0, ty1 => fun n l => n < length l
-  | ty1, ty0 => fun l n => length l < n
-  end a b.
+(** We first declare the prototypes ouf our mutual definitions. *)
+Set Universe Polymorphism.
+Inductive ty : forall (A : Type) (P : A -> Type), Set :=
+| ty0 : ty nat (fun _ => nat)
+| ty1 : ty (list nat) (fun _ => bool).
+Derive Signature NoConfusion for ty.
 
-Polymorphic Instance: WellFounded rel.
-Proof. Admitted.
-Require Import Arith.
+(** Our measure is simple, just the natural number or length of the list argument. *)
+Equations measure : {A &{ P &{ _ : A & ty A P }}} -> nat :=
+  measure &(_, _, a, ty0) => a;
+  measure &(_, _, a, ty1) => length a.
 
-Polymorphic Definition pack {A} {P} (x : A) (t : ty A P) :=
-  (&(A, P, x, t)) : {A & {P & {_ : A & ty A P}}}.
+Definition rel := MR lt measure.
 
-Polymorphic Equations? double_fn {A} {P} (t : ty A P) (x : A) : P x by rec (pack x t) rel :=
+Instance: WellFounded rel.
+Proof.
+  red. apply measure_wf. apply Wf_nat.lt_wf.
+Defined.
+
+Definition pack {A} {P} (x : A) (t : ty A P) := (&(A, P, x, t)) : {A & {P & {_ : A & ty A P}}}.
+
+(** We define the function by recursion on the abstract packed argument.
+    Using dependent pattern matching, the clauses for [ty0] refine the argument
+    and return type to [nat] and similarly for [ty1], we can hence do pattern-matching
+    as usual on each separate definition. *)
+Equations? double_fn {A} {P} (t : ty A P) (x : A) : P x by rec (pack x t) rel :=
   double_fn ty0 n := n + 0;
   double_fn ty1 nil := true;
   double_fn ty1 (x :: xs) := 0 <? length xs + double_fn ty0 (length xs).
-Proof. Transparent rel. unfold rel. simp rel. cbn. auto with arith. Qed.
+(** It is easily shown terminating in this case. *)
+Proof. red. red. cbn. auto with arith. Qed.
 
+(** We can define auxilliary definition to select the functions we want and express unfolding
+    lemmas in terms of these abbreviations. *)
 Definition fn0 := double_fn ty0.
 Definition fn1 := double_fn ty1.
 
@@ -59,156 +73,5 @@ Qed.
 
 Lemma fn1_unfold l : fn1 l = match l with nil => true | x :: xs => 0 <? length xs + fn0 (length xs) end.
 Proof.
-  unfold fn1; simp double_fn. destruct l. simp double_fn. simp double_fn. now rewrite fn0_unfold.
+  unfold fn1; simp double_fn. destruct l. simp double_fn. simp double_fn.
 Qed.
-
-(* Polymorphic Equations double_fn' {A} {P} (t : ty A P) (x : A) : P x by rec (pack x t) rel := *)
-(*   double_fn' ty0 n := n + 0; *)
-(*   double_fn' ty1 l := aux l _ *)
-(*     where aux l' (H : length l' <= length l)  : _ by struct l' := *)
-(*     aux nil _ := true; *)
-(*     aux (x :: xs) H := 0 <? length xs + double_fn' ty0 (length xs) + if aux xs _ then 0 else 1. *)
-(* Obligation Tactic := idtac. *)
-(* Next Obligation. intros. cbn. auto with arith. Defined. *)
-(* Next Obligation. intros. cbn. auto with arith. Defined. *)
-(* Next Obligation. auto with arith. Defined. *)
-
-(* Definition fn0' := Eval compute in double_fn' ty0. *)
-(* Definition fn1' := double_fn' ty1. *)
-
-(* Lemma fn0'_unfold n : fn0' n = n + 0. *)
-(* Proof. *)
-(*   unfold fn0'; simp double_fn'. *)
-(* Qed. *)
-
-(* Lemma fn1'_unfold l : fn1' l = match l with nil => true | x :: xs => 0 <? length xs + fn0' (length xs) end. *)
-(* Proof. *)
-(*   unfold fn1'; simp double_fn'. destruct l. simp double_fn. simp double_fn'. *)
-(*   destruct double_fn'_unfold_obligation_1. rewrite fn0'_unfold.  auto. *)
-(*   rewrite fn0'_unfold. *)
-(* Admitted. *)
-
-Require Import Equations.Subterm.
-Obligation Tactic := program_simpl; try typeclasses eauto 10 with Below.
-
-Equations ack (m n : nat) : nat by rec (m, n) (lexprod _ _ lt lt) :=
-  ack 0 0         := 1;
-  ack 0 (S n)     := S (S n);
-  ack (S m) 0     := ack m 1;
-  ack (S m) (S n) := ack m (ack (S m) n).
-
-Module Abc.
-
-Inductive abc : Set :=
-| abc0
-  | A (a : abc)
-  | B (b : abc)
-  | C (c : abc).
-
-(* Inductive sct0_rel : abc -> abc -> Prop := *)
-(* | sct0_bc x : sct0_rel (B (C x)) (A x) *)
-(* | sct0_a x : sct0_rel x (A x) *)
-(* | sct0_b x : sct0_rel x (B x) *)
-(* | sct0_c x : sct0_rel x (C x). *)
-(* Hint Constructors sct0_rel : rec_decision. *)
-(* Instance: WellFounded sct0_rel. *)
-(* Admitted. *)
-
-Fixpoint measure_abc (x : abc) :=
-  match x with
-  | abc0 => 0
-  | A x => 3 + measure_abc x
-  | B x => S (measure_abc x)
-  | C x => S (measure_abc x)
-  end.
-
-
-Equations sct0 (x : abc) : nat by rec (measure_abc x) lt :=
-  sct0 abc0 := 0;
-  sct0 (A x) := sct0 (B (C x)) + sct0 x;
-  sct0 (B x) := sct0 x;
-  sct0 (C x) := sct0 x.
-
-Fixpoint measure_abc' (x : abc) :=
-  match x with
-  | abc0 => 0
-  | A x => S (measure_abc' x)
-  | B x => S (measure_abc' x)
-  | C x => S (measure_abc' x)
-  end.
-
-Equations? f1g1 (x : abc) : unit by rec (measure_abc' x) lt :=
-  f1g1 (A (A x)) := f1 x _
-    where f1 x' (H : measure_abc' x' < measure_abc' (A x)) : _ := { f1 x _ := f1g1 (A x) };
-  f1g1 _ := tt.
-Proof. auto with arith. Defined.
-
-Equations f1g1' (x : abc) : unit by rec (measure_abc' x) lt :=
-  f1g1' (A (A x)) := f1g1' (A x);
-  f1g1' _ := tt.
-End Abc.
-
-Module sct2.
-
-  Polymorphic Inductive ty : forall (A : Type) (P : A -> Type), Type :=
-  | ty0 : ty (list nat * list nat)%type (fun _ => list nat)
-  | ty1 : ty (list nat * list nat * list nat) (fun _ => list nat).
-
-  Definition type := {A &{ P &{ _ : ty A P & A }}}.
-
-  (* Equations measure (x : type) : nat := *)
-  (*   measure &(_, _, ty0, (l, l')) := length l; *)
-  (*   measure &(_, _, ty1, (l, l', l'')) := length l. *)
-
-  Polymorphic Equations rel' : {A &{ P &{ _ : ty A P & A }}} -> {A & { P & {_ : ty A P & A}}} -> Prop :=
-  rel' &(A', P, ta, a) &(_, Q, tb, b) =>
-  match ta in ty A P, tb in ty B Q return A -> B -> Prop with
-  | ty0, ty0 => fun '(l0, l1) '(l0', l1') => (* length l0 < length l0' *) False
-  | ty1, ty1 => fun '(l0, n, l1) '(l0', n', l1') => (* length l0 < length l0' *) False
-  | ty0, ty1 => fun '(l0, l1) '(l0', l1', l2') => length l0 <= length l0'
-  | ty1, ty0 => fun '(l0, l1, l2) '(l0', l1') => length l0 < length l0'
-  end a b.
-
-  Transparent rel'.
-  Polymorphic Instance: WellFounded rel'.
-  Proof. Admitted.
-    (* red. intros a. dependent elimination a as [&(A, P, ta, a)]. *)
-    (* simpl in *. constructor. intros y. *)
-    (* dependent elimination y as [&(A', P', tb, a')]; *)
-    (* simpl in *. *)
-    (* intros rel'. unfold sct2.rel' in rel'. destruct tb. destruct ta; simpl in *. *)
-    (* simpl in *. destruct a, a'. simpl in *. destruct rel'. *)
-    (* destruct a, a'. destruct p. *)
-    (* constructor. intros (A'&P'&t'&a'). *)
-
-  Polymorphic Definition pack {A} {P} (t : ty A P) (x : A) :=
-  (&(A, P, t, x)) : {A & {P & {_ : ty A P & A}}}.
-
-  Obligation Tactic := program_simpl; unfold rel'; cbn; auto with arith.
-
-  Polymorphic Equations fg {A} {P} (t : ty A P) (x : A) : P x by rec (pack t x) rel' :=
-    fg ty0 (nil, x) := x;
-    fg ty0 (cons y ys, x) := 1 :: fg ty1 (ys, x, (cons y ys));
-    fg ty1 (a, b, c) := 2 :: fg ty0 (a, app b c).
-
-  Inductive fg_dom : forall (A : Set) (P : A -> Set), ty A P -> A -> Prop :=
-  | fg_dom_equation_1 :
-      forall l0 : list nat,
-        fg_dom (list nat * list nat) (fun _ : list nat * list nat => list nat) ty0 (nil, l0)
-  | fg_dom_equation_2 : forall (n : nat) (l l0 : list nat),
-      fg_dom (list nat * list nat * list nat)
-             (fun _ : list nat * list nat * list nat => list nat) ty1 (l, l0, n :: l) ->
-
-      fg_dom (list nat * list nat) (fun _ : list nat * list nat => list nat) ty0
-                          (n :: l, l0)
-  | fg_dom_equation_3 : forall l0 l1 l : list nat,
-                        fg_dom (list nat * list nat) (fun _ : list nat * list nat => list nat) ty0
-                          (l0, l1 ++ l) ->
-                        fg_dom (list nat * list nat * list nat)
-                          (fun _ : list nat * list nat * list nat => list nat) ty1 (l0, l1, l).
-
-  (* Lemma fg_ind_inh : forall A P t x, fg_dom A P t x. *)
-  (* Proof. *)
-  (*   intros. *)
-
-End sct2.
