examples/wfrec.v
@@ -75,3 +75,12 @@ Proof.
   destruct (proj2 Heq). reflexivity. discriminate.
   auto.
 Qed.
+
+Require Import Equations.Subterm.
+Obligation Tactic := program_simpl; try typeclasses eauto 10 with Below.
+
+Equations ack (m n : nat) : nat by rec (m, n) (lexprod _ _ lt lt) :=
+  ack 0 0         := 1;
+  ack 0 (S n)     := S (S n);
+  ack (S m) 0     := ack m 1;
+  ack (S m) (S n) := ack m (ack (S m) n).
